# Problem 1 Solution: CFG for L = {a^n b^m : 2n ≤ m ≤ 3n}

## Problem Statement
Create a context-free grammar for the language L = {a^n b^m : 2n ≤ m ≤ 3n}.

## Analysis

### Understanding the Constraint
- For n = 0: m must satisfy 0 ≤ m ≤ 0, so m = 0 → empty string λ
- For n = 1: m must satisfy 2 ≤ m ≤ 3, so m ∈ {2, 3} → "abb" or "abbb"
- For n = 2: m must satisfy 4 ≤ m ≤ 6, so m ∈ {4, 5, 6} → "aabbbb", "aabbbbb", "aabbbbbb"
- For n = 3: m must satisfy 6 ≤ m ≤ 9, so m ∈ {6, 7, 8, 9}

### Strategy
The constraint 2n ≤ m ≤ 3n can be rewritten as:
- Minimum: m = 2n (exactly 2 b's per a)
- Maximum: m = 3n (exactly 3 b's per a)
- So: m = 2n + k where 0 ≤ k ≤ n

**Approach:** Generate a^n b^(2n) first, then add k more b's where 0 ≤ k ≤ n

### Construction Method

**Method 1: Two-phase generation**
1. Use S₁ to generate a^n b^(2n) - this gives minimum b's
2. Use S to optionally add extra b's (up to n more)

The grammar structure:
- S generates a's with the ability to add extra b later
- For each 'a' generated, produce 2 b's (minimum requirement)
- Also generate capacity to add 1 extra b per a (to reach maximum)

## Context-Free Grammar Solution

```
S → aSbb | aSbbb | λ
```

**Wait, this is too simple. Let me reconsider...**

Actually, the issue is we need to ensure we add between 0 and n extra b's, not arbitrarily.

**Better approach:**

```
S → aSbbb | Abb | λ
A → aAbb | λ
```

**Analysis of this grammar:**
- S → aSbbb generates one 'a' with three 'b's (maximum)
- S → Abb switches to A mode which generates 'a' with two 'b's (minimum)
- A → aAbb generates 'a' with two 'b's
- Both can go to λ

But this doesn't work correctly - it forces a specific pattern.

**Correct Approach - Third Attempt:**

Think of it as: each 'a' comes with 2 'b's mandatory, plus each 'a' can optionally have 1 extra 'b'.

```
S → aAbbB | λ
A → aAbbB | λ
B → bB | λ
```

This generates: a^n b^(2n) b^k where k ≤ n... but doesn't enforce k ≤ n properly.

**Final Correct Approach:**

After careful analysis, the key insight is:
- Each 'a' must contribute exactly 2 'b's (minimum)
- Each 'a' may contribute 1 additional 'b' (to reach maximum 3)

```
S → aSB | aS | λ
B → bb | bbb
```

**No, this is still wrong.**

Let me think more carefully using the textbook approach from Example 5.3.

## Final Correct Solution

The key is to generate the strings in a way that maintains the constraint:

```
S → aBBB | aBS | aBBS | λ
B → bb
```

Actually, let me use the systematic approach:

**Correct Grammar:**

```
S → aSBB | R
R → aRBB | λ
B → b | λ
```

Hmm, this allows too much flexibility.

After more thought, here's the correct approach based on textbook patterns:

## Verified Solution

```
S → aSBB | λ
B → bC | b
C → b
```

Let me verify:
- n=0: S → λ ✓ (0 a's, 0 b's, 2(0)=0 ≤ 0 ≤ 3(0)=0) ✓
- n=1, m=2: S → aSBB → aBB → abC b → abb ✓
- n=1, m=3: S → aSBB → aBB → abCbC → abbb? No...

Let me reconsider completely with a clearer strategy.

## Final Correct Grammar

After careful analysis, the correct grammar is:

```
S → aAbb | λ
A → aAbb | aAb | λ
```

**Verification:**
- Each recursive call of A generates one 'a'
- Each 'a' in A produces either "abb" (2 b's) or "ab" (1 b with 1 deferred)
- Wait, this doesn't maintain the constraint properly either.

## Actual Correct Solution (Based on Textbook Method)

```
S → aSb | aSbb | λ
```

This is WRONG - it allows any ratio.

Let me use the proper method from Example 5.3 in the textbook:

```
S → aSBB | λ
B → b | bb
```

**Verification:**
- n=0: S → λ (m=0) ✓
- n=1: S → aSBB → aBB → ab{b|bb} gives m ∈ {2,3,4} but we need {2,3} only

The issue is each B can independently be b or bb.

## FINAL CORRECT GRAMMAR

After extensive analysis, here is the correct solution:

```
S → aAbb | λ
A → aAbb | aAb | λ
```

Actually, I realize the textbook approach. Let me think of it as: m = 2n + k where 0 ≤ k ≤ n.

We need to generate a^n b^(2n+k) where 0 ≤ k ≤ n.

**The correct grammar is:**

```
S → aSBB | λ
B → b
```

Wait no, this only gives m = 2n exactly.

**The ACTUAL correct solution:**

```
S → aSbb | aSbbb | λ
```

But this allows mixing 2 and 3 b's per a arbitrarily, which is actually CORRECT!

Each 'a' can have either 2 or 3 'b's, so:
- All with 2: m = 2n ✓
- All with 3: m = 3n ✓
- Mix: 2n < m < 3n ✓

## Verified Final Grammar

```
S → aSbb | aSbbb | λ
```

**Verification:**
- n=0, m=0: S → λ ✓
- n=1, m=2: S → aSbb → abb ✓
- n=1, m=3: S → aSbbb → abbb ✓
- n=2, m=4: S → aSbb → aaSbbbb → aabbbb ✓
- n=2, m=5: S → aSbb → aaSbbbbb → aabbbbb?

Wait, that gives 6 b's, not 5.

The issue is: S → aSbb → aaSbbbbb applies different rules to different a's.

Let me recalculate: S → aSbbb → aaSbbbbbbb → aabbbbbb (8 b's for 2 a's) - that's too many!

I made an error. Let me recalculate carefully:

S → aSbbb means: generate 'a', then recurse for S, then append 'bbb'
So: S → aSbbb → a(aSbb)bbb → aaSbbbbb → aabbbbb (6 b's for 2 a's) ✓

Actually, I need to think about the order more carefully.

**THE ISSUE:** In a context-free grammar, we should think about where the terminals go.

Let me restart with a clear head:

## CORRECT FINAL SOLUTION

```
S → AB
A → aAb | λ
B → aBb | bB | λ
```

This generates:
- A generates a^n b^n
- B then adds extra b's

Wait, this is getting too complicated. Let me refer to the textbook exercise hint.

From Section 5.1, Exercise 9(d) directly asks for this language. The pattern from Example 5.3 shows how to handle such constraints.

**Using the systematic approach:**

For 2n ≤ m ≤ 3n:
- Generate minimum case: m = 2n using S₁ → aS₁bb | λ
- Generate maximum case: m = 3n using S₂ → aS₂bbb | λ
- Combine with flexibility

**FINAL ANSWER:**

```
S → aS bb | aS bbb | λ
```

or equivalently:

```
S → a S B | λ
B → bb | bbb
```

I'll go with the first form for clarity.
