# Problem 1 Final Solution

## Problem
Create a context-free grammar for L = {a^n b^m : 2n ≤ m ≤ 3n}

## Solution

### Context-Free Grammar:
```
S → aSbb | aSbbb | λ
```

or equivalently written as:

```
S → aSB | λ
B → bb | bbb
```

I'll use the first form for the final answer.

## Explanation

The constraint 2n ≤ m ≤ 3n means:
- For each 'a', we need at least 2 'b's and at most 3 'b's
- We can choose freely for each 'a' whether it "contributes" 2 or 3 'b's

### How the Grammar Works:

1. **Production S → aSbb**:
   - Generates one 'a' followed by exactly 2 'b's
   - Then recurses with S

2. **Production S → aSbbb**:
   - Generates one 'a' followed by exactly 3 'b's
   - Then recurses with S

3. **Production S → λ**:
   - Base case (terminates the recursion)

### Key Insight:
By allowing each recursive step to choose between adding "abb" or "abbb", we can generate any string where the total number of b's is between 2n and 3n for n a's.

## Verification

**n = 0, m = 0:**
S ⇒ λ
String: λ (empty string)
Check: 2(0) = 0 ≤ 0 ≤ 0 = 3(0) ✓

**n = 1, m = 2:**
S ⇒ aSbb ⇒ abb
Check: 2(1) = 2 ≤ 2 ≤ 3 = 3(1) ✓

**n = 1, m = 3:**
S ⇒ aSbbb ⇒ abbb
Check: 2(1) = 2 ≤ 3 ≤ 3 = 3(1) ✓

**n = 2, m = 4:**
S ⇒ aSbb ⇒ aaSbbbb ⇒ aabbbb
Check: 2(2) = 4 ≤ 4 ≤ 6 = 3(2) ✓

**n = 2, m = 5:**
S ⇒ aSbb ⇒ aaSbbbbb ⇒ aabbbbb
Check: 2(2) = 4 ≤ 5 ≤ 6 = 3(2) ✓

**n = 2, m = 6:**
S ⇒ aSbbb ⇒ aaSbbbbbb ⇒ aabbbbbb
Check: 2(2) = 4 ≤ 6 ≤ 6 = 3(2) ✓

**Invalid example - n = 2, m = 3:**
Cannot be generated (and correctly so, since 3 < 2(2) = 4)

**Invalid example - n = 2, m = 7:**
Cannot be generated (and correctly so, since 7 > 3(2) = 6)

## Formal Proof of Correctness

**Claim:** L(G) = {a^n b^m : 2n ≤ m ≤ 3n}

**Proof:**

**(⊆ direction)** Every string generated by G is in the language:
- By induction on derivation length
- Base case: λ is generated by S → λ, and satisfies 2(0) ≤ 0 ≤ 3(0) ✓
- Inductive step: If S ⇒* a^n b^m with 2n ≤ m ≤ 3n, then:
  - S ⇒ aSbb ⇒* aa^n bb^m = a^(n+1) b^(m+2), and 2(n+1) ≤ m+2 ≤ 3(n+1)
    since 2n+2 ≤ m+2 ≤ 3n+2 which follows from 2n ≤ m ≤ 3n
  - Similarly for S → aSbbb

**(⊇ direction)** Every string in the language can be generated:
- Given a^n b^m with 2n ≤ m ≤ 3n, we can write m = 2k + 3(n-k) for some 0 ≤ k ≤ n
- Use S → aSbb k times and S → aSbbb (n-k) times
- This generates a^n b^(2k + 3(n-k)) = a^n b^m

Therefore, L(G) = {a^n b^m : 2n ≤ m ≤ 3n}. ∎
